Wavelet/Simulation/Ret.lean
@@ -14,154 +14,12 @@ namespace Wavelet.Simulation.Ret
 open Wavelet.Op Wavelet.Seq Wavelet.Dataflow Wavelet.Compile
 open Relation Lemmas
 
-theorem expr_outputs_nodup :
-  (compileExpr.exprOutputs χ m n pathConds).toList.Nodup
-:= by
-  simp only [
-    compileExpr.exprOutputs, Vector.toList_append, Vector.toList_push,
-    Vector.toList_map, Vector.toList_range]
-  apply List.Nodup.append
-  · apply List.Nodup.map _ List.nodup_range
-    simp [Function.Injective]
-  · apply List.Nodup.append
-    · apply List.Nodup.map _ List.nodup_range
-      simp [Function.Injective]
-    · simp
-    · simp
-  · simp
-    apply List.disjoint_iff_ne.mpr
-    simp
-
-theorem exprOutputs_finIdxOf?_tail_cond :
-  (compileExpr.exprOutputs _ m n pathConds).finIdxOf?
-    (.tail_cond pathConds) = some (⟨n + m, by simp⟩)
-  := by
-  simp only [compileExpr.exprOutputs]
-  apply Vector.finIdxOf?_eq_some_iff.mpr
-  constructor
-  · simp [Vector.get_eq_getElem]
-  · intros j hj hget
-    simp [Vector.get_eq_getElem, Vector.getElem_append] at hget
-    split at hget
-    · simp at hget
-    · simp [Vector.getElem_push] at hget
-      omega
-
-theorem exprOutputs_finIdxOf?_tail_args
-  (hi : i < m) :
-  (compileExpr.exprOutputs _ m n pathConds).finIdxOf?
-    (.tail_arg i pathConds) = some (⟨n + i, by omega⟩)
-  := by
-  simp [compileExpr.exprOutputs]
-  constructor
-  · simp [Vector.get_eq_getElem, hi]
-  · intros j hj hget
-    simp [Vector.get_eq_getElem, Vector.getElem_append] at hget
-    split at hget <;> rename_i h
-    · simp at hget
-    · simp [Vector.getElem_push] at hget
-      split at hget
-      · simp [Fin.lt_def] at hj
-        simp at hget
-        omega
-      · simp at hget
-
-theorem exprOutputs_finIdxOf?_dest
-  (hi : i < n) :
-  (compileExpr.exprOutputs _ m n pathConds).finIdxOf?
-    (.dest i pathConds) = some (⟨i, by omega⟩)
-  := by
-  simp [compileExpr.exprOutputs]
-  constructor
-  · simp [Vector.get_eq_getElem, hi]
-  · intros j hj hget
-    simp [Vector.get_eq_getElem, Vector.getElem_append] at hget
-    split at hget <;> rename_i h
-    · simp [Fin.lt_def] at hj
-      simp at hget
-      omega
-    · simp [Vector.getElem_push] at hget
-      split at hget
-      · simp [Fin.lt_def] at hj
-        simp at hget
-      · simp at hget
-
-theorem exprOutputs_finIdxOf?_no_match_dest
-  {pathConds pathConds' : List (Bool × ChanName χ)}
-  (hi : i < n → pathConds' ≠ pathConds) :
-  (compileExpr.exprOutputs _ m n pathConds).finIdxOf?
-    (.dest i pathConds') = none
-  := by
-  if h : i < n then
-    simp [compileExpr.exprOutputs, Ne.symm (hi h)]
-  else
-    simp [compileExpr.exprOutputs, h]
-
-theorem exprOutputs_finIdxOf?_no_match_tail_args
-  {pathConds pathConds' : List (Bool × ChanName χ)}
-  (hi : i < m → pathConds' ≠ pathConds) :
-  (compileExpr.exprOutputs _ m n pathConds).finIdxOf?
-    (.tail_arg i pathConds') = none
-  := by
-  if h : i < m then
-    simp [compileExpr.exprOutputs, Ne.symm (hi h)]
-  else
-    simp [compileExpr.exprOutputs, h]
-
-theorem exprOutputs_finIdxOf?_no_match_tail_cond
-  {pathConds pathConds' : List (Bool × ChanName χ)}
-  (h : pathConds' ≠ pathConds) :
-  (compileExpr.exprOutputs _ m n pathConds).finIdxOf?
-    (.tail_cond pathConds') = none
-  := by simp [compileExpr.exprOutputs, h]
-
-@[simp]
-private theorem exprOutputs_finIdxOf?_no_match_var :
-  (compileExpr.exprOutputs _ m n pathConds).finIdxOf?
-    (.var v pathConds') = none
-  := by simp [compileExpr.exprOutputs]
-
-@[simp]
-private theorem exprOutputs_finIdxOf?_no_match_merge_cond :
-  (compileExpr.exprOutputs _ m n pathConds).finIdxOf?
-    (.merge_cond condName) = none
-  := by simp [compileExpr.exprOutputs]
-
-@[simp]
-theorem exprOutputs_finIdxOf?_no_match_tail_cond_carry :
-  (compileExpr.exprOutputs _ m n pathConds).finIdxOf?
-    .tail_cond_carry = none
-  := by simp [compileExpr.exprOutputs]
-
-@[simp]
-private theorem exprOutputs_finIdxOf?_no_match_tail_cond_steer_dests :
-  (compileExpr.exprOutputs _ m n pathConds).finIdxOf?
-    .tail_cond_steer_dests = none
-  := by simp [compileExpr.exprOutputs]
-
-@[simp]
-private theorem exprOutputs_finIdxOf?_no_match_tail_cond_steer_tail_args :
-  (compileExpr.exprOutputs _ m n pathConds).finIdxOf?
-    .tail_cond_steer_tail_args = none
-  := by simp [compileExpr.exprOutputs]
-
-@[simp]
-private theorem exprOutputs_finIdxOf?_no_match_final_dest :
-  (compileExpr.exprOutputs _ m n pathConds).finIdxOf?
-    (.final_dest i) = none
-  := by simp [compileExpr.exprOutputs]
-
-theorem path_conds_nodup_alt
-  (hnodup : (pathConds.map Prod.snd).Nodup)
-  (hpath_conds : ((b, condName) :: tailConds).Sublist pathConds) :
-  (b', condName) ∉ tailConds := by grind
-
 universe u
 variable (Op : Type u) (χ : Type u) (V S)
 variable [instArity : Arity Op] [DecidableEq χ] [instInterp : Interp Op V S]
 
 /-- Values pushed to output channels in the case of a return. -/
-def exprOutputVals
+private def exprOutputVals
   (retVals : Vector V n)
   : Vector V (n + (m + 1)) :=
   retVals ++
@@ -173,7 +31,7 @@ have fired, but before the `merge`s finish. -/
 def intermChans
   (ec : Seq.Config Op χ V S m n)
   (_pc : Dataflow.Config Op (ChanName χ) V S m n)
-  (clearVars : Vector χ n)
+  (clearVars : Vector χ k)
   (vals : Vector V (n + (m + 1)))
   (pathConds : List (Bool × ChanName χ))
   (name : ChanName χ)
@@ -250,7 +108,7 @@ theorem sim_step_ret_merges
         | .tail_arg _ _ => val = Interp.junkVal (self := instInterp) Op S
         | .tail_cond _ => val = instInterp.fromBool false
         | _ => False)
-      (by apply expr_outputs_nodup)
+      (by apply exprOutputs_nodup)
       (by
         intros name hname
         simp [hchans₁, intermChans]
@@ -310,7 +168,7 @@ theorem sim_step_ret_merges
     -- Simplify pushes
     rw [push_vals_empty] at hstep
     rotate_left
-    · apply expr_outputs_nodup
+    · apply exprOutputs_nodup
     · intros name hname
       -- simp [compileExpr.exprOutputs] at hname
       simp [hchans₂, hchans₁, intermChans]
@@ -447,7 +305,7 @@ theorem sim_step_ret_forwardc_sink
   -- Simplify pushes
   rw [push_vals_empty] at hsteps₁
   rotate_left
-  · apply expr_outputs_nodup
+  · apply exprOutputs_nodup
   · intros name hmem_name
     simp at hmem_name
     simp [hchans₁, ← hvar_names, compileExpr.varNames,
@@ -465,11 +323,11 @@ theorem sim_step_ret_forwardc_sink
     (map := pc₁.chans)
     (names := compileExpr.allVarsExcept χ ec.definedVars vars.toList ec.pathConds)
     (λ name val => True)
-    (allVarsExcept_nodup _ hdefined_vars_no_dup)
+    (allVarsExcept_nodup hdefined_vars_no_dup)
     (by
       simp
       intros name hname
-      have ⟨var, hvar, hmem_var, hnot_mem_var⟩ := mem_allVarsExcept _ hname
+      have ⟨var, hvar, hmem_var, hnot_mem_var⟩ := mem_allVarsExcept hname
       simp [hvar, hpc₁]
       simp [hlive_vars, SimR.varsToChans]
       have ⟨val, h⟩ := (hdefined_vars var).mp hmem_var
@@ -489,7 +347,7 @@ theorem sim_step_ret_forwardc_sink
   funext name
   simp [intermChans, hchans₂, hpc₁]
   split <;> rename_i h₁
-  · have ⟨var, hvar, hmem_var, hnot_mem_var⟩ := mem_allVarsExcept _ h₁
+  · have ⟨var, hvar, hmem_var, hnot_mem_var⟩ := mem_allVarsExcept h₁
     simp [hvar]
   · split <;> rename_i h₂
     · simp [h₂, ← hjunk, ← hfalse, exprOutputVals]
@@ -506,7 +364,7 @@ theorem sim_step_ret_forwardc_sink
           simp [compileExpr.allVarsExcept, List.toVector] at h₁
           split <;> rename_i h₄
           · replace h₄ := (hdefined_vars var').mpr ⟨_, h₄⟩
-            have := h₁ (mem_to_mem_removeAll h₄ (by simp [h₃]))
+            have := h₁ (List.mem_to_mem_removeAll h₄ (by simp [h₃]))
             simp [h] at this
           · rfl
         | merge_cond condName => rfl
