Wavelet/Simulation.lean
@@ -1,4 +1,5 @@
 import Wavelet.Simulation.Relation
-import Wavelet.Simulation.Br
 import Wavelet.Simulation.Ret
+import Wavelet.Simulation.Tail
 import Wavelet.Simulation.Op
+import Wavelet.Simulation.Br
