Wavelet/Simulation/Tail.lean
@@ -1,0 +1,199 @@
+import Mathlib.Data.Vector.Basic
+
+import Wavelet.Op
+import Wavelet.Seq
+import Wavelet.Dataflow
+import Wavelet.Compile
+import Wavelet.Lemmas
+
+import Wavelet.Simulation.Relation
+import Wavelet.Simulation.Lemmas
+import Wavelet.Simulation.Ret
+
+namespace Wavelet.Simulation.Tail
+
+open Wavelet.Op Wavelet.Seq Wavelet.Dataflow Wavelet.Compile
+open Relation Lemmas Ret
+
+universe u
+variable (Op : Type u) (χ : Type u) (V S)
+variable [instArity : Arity Op] [DecidableEq χ] [instInterp : Interp Op V S]
+
+/-- Values pushed to output channels in the case of a tail call. -/
+private def exprOutputVals
+  (tailArgs : Vector V m)
+  : Vector V (n + (m + 1)) :=
+  Vector.replicate n (Interp.junkVal Op S : V) ++
+  tailArgs.push
+  (Interp.fromBool Op S true)
+
+set_option maxHeartbeats 300000
+
+/-- Fires `forwardc` and `sink` to get an intermediate state. -/
+theorem sim_step_tail_forwardc_sink
+  (hnz : m > 0 ∧ n > 0)
+  {ec : Seq.Config Op χ V S m n}
+  {pc : Dataflow.Config Op (ChanName χ) V S m n}
+  (hsim : SimR _ _ _ _ hnz ec pc)
+  (hexpr : ec.expr = .cont (.tail vars))
+  (hvars : VarMap.getVars χ V vars ec.vars = some tailArgs)
+  (hvars_nodup : vars.toList.Nodup) :
+  Dataflow.Config.StepPlus Op (ChanName χ) V S pc
+  { proc := pc.proc,
+    chans := intermChans _ _ _ _ ec pc vars
+      (exprOutputVals Op V S tailArgs)
+      ec.pathConds
+    state := pc.state }
+:= by
+  have ⟨
+    heq_state,
+    hlive_vars,
+    hdefined_vars_no_dup,
+    hdefined_vars,
+    hpath_conds_order,
+    hpath_conds_nodup,
+    hmerges,
+    ⟨
+      rest, carryInLoop, ctxLeft, ctxCurrent, ctxRight,
+      hatoms,
+      hcomp_fn,
+      hrest,
+      hret,
+      hcont,
+    ⟩,
+  ⟩ := hsim
+  have ⟨hcarryInLoop, hwf_expr, hcurrent⟩ := hcont _ hexpr
+  simp [compileExpr] at hcurrent
+  -- Some abbreviations
+  generalize hvar_names :
+    compileExpr.varNames χ ec.pathConds vars = varNames
+  generalize hjunk :
+    Interp.junkVal (self := instInterp) Op S = junk
+  generalize htrue :
+    Interp.fromBool (self := instInterp) Op S true = trueVal
+  simp only [hvar_names, hjunk, htrue] at hcurrent
+  -- Step 1: Fire `forwardc`.
+  have ⟨chans₁, tailArgs', hpop_tail_args, hchans₁, htail_args⟩ :=
+    pop_vals_singleton _ _
+    (map := pc.chans)
+    (names := varNames)
+    (λ name val =>
+      ∃ var,
+        name = .var var ec.pathConds ∧
+        ec.vars.getVar _ _ var = some val)
+    (by
+      simp only [← hvar_names, compileExpr.varNames, Vector.toList_map]
+      apply List.Nodup.map _ hvars_nodup
+      simp [Function.Injective, compileExpr.varName])
+    (by
+      simp [← hvar_names, hlive_vars, compileExpr.varNames,
+        compileExpr.varName, SimR.varsToChans]
+      have := Vector.mapM_some_implies_all_some hvars
+      intros v hmem_v
+      have ⟨val, _, hval⟩ := this v hmem_v
+      exists val
+      simp [VarMap.getVar, hval])
+  have heq_ret_vals :
+    tailArgs' = tailArgs
+  := by
+    apply Vector.toList_inj.mp
+    apply List.right_unique_forall₂' _ htail_args
+    · simp [← hvar_names, compileExpr.varNames, compileExpr.varName,
+        Vector.toList_map, VarMap.getVar]
+      apply List.mapM_some_iff_forall₂.mp (Vector.mapM_toList hvars)
+    · simp [Relator.RightUnique, VarMap.getVar]
+      grind
+  replace heq_ret_vals := heq_ret_vals.symm
+  subst heq_ret_vals
+  have hmem_forwardc :
+    AtomicProc.forwardc
+      varNames ((Vector.replicate n junk).push trueVal)
+      (compileExpr.exprOutputs' χ m n ec.pathConds)
+      ∈ pc.proc.atoms
+  := by grind
+  have hsteps₁ : Dataflow.Config.StepPlus _ _ _ _ pc _
+    := Relation.TransGen.single (Dataflow.Config.Step.step_forwardc hmem_forwardc hpop_tail_args)
+  -- Simplify pushes
+  rw [push_vals_empty] at hsteps₁
+  rotate_left
+  · apply exprOutputs'_nodup
+  · intros name hmem_name
+    simp at hmem_name
+    simp [hchans₁, ← hvar_names, compileExpr.varNames,
+      compileExpr.varName, hlive_vars, SimR.varsToChans]
+    simp [compileExpr.exprOutputs'] at hmem_name
+    rcases hmem_name with ⟨_, _, h⟩ | ⟨_, _, h⟩ | h
+    · simp [← h]
+    · simp [← h]
+    · simp [h]
+  simp only [hchans₁] at hsteps₁
+  replace ⟨pc₁, hpc₁, hsteps₁⟩ := exists_eq_left.mpr hsteps₁
+  -- Step 2: Fire `sink` to consume all unused channels in the current context.
+  have ⟨chans₂, otherVals, hpop_other_vals, hchans₂, hother_vals⟩ :=
+    pop_vals_singleton _ _
+    (map := pc₁.chans)
+    (names := compileExpr.allVarsExcept χ ec.definedVars vars.toList ec.pathConds)
+    (λ name val => True)
+    (allVarsExcept_nodup hdefined_vars_no_dup)
+    (by
+      simp
+      intros name hname
+      have ⟨var, hvar, hmem_var, hnot_mem_var⟩ := mem_allVarsExcept hname
+      simp [hvar, hpc₁]
+      simp [hlive_vars, SimR.varsToChans]
+      have ⟨val, h⟩ := (hdefined_vars var).mp hmem_var
+      exists val
+      simp at hnot_mem_var
+      simp [h, ← hvar_names, compileExpr.varNames, compileExpr.varName, hnot_mem_var])
+  have hmem_sink :
+    .sink (compileExpr.allVarsExcept χ ec.definedVars vars.toList ec.pathConds)
+    ∈ pc₁.proc.atoms
+  := by grind
+  have hsteps₂ : Dataflow.Config.StepPlus _ _ _ _ pc _
+    := Relation.TransGen.tail hsteps₁
+      (Dataflow.Config.Step.step_sink hmem_sink hpop_other_vals)
+  apply step_plus_eq
+  apply hsteps₂
+  simp [hpc₁]
+  funext name
+  simp [intermChans, hchans₂, hpc₁]
+  split <;> rename_i h₁
+  · have ⟨var, hvar, hmem_var, hnot_mem_var⟩ := mem_allVarsExcept h₁
+    simp [hvar]
+  · split <;> rename_i h₂
+    · simp [exprOutputs'_finIdxOf?_some_to_exprOutputs h₂, ← hjunk, ← htrue, exprOutputVals]
+      -- Rearrange positions of tail arguments and return values
+      rename_i i
+      split_ifs <;> rename_i h₃
+      · simp [h₃]
+      · rename_i h₄
+        have : ↑i - m < n := by omega
+        simp [Vector.getElem_push, Vector.getElem_append]
+        simp [h₄, this]
+      · rename_i h₄
+        simp at h₃
+        simp [Vector.getElem_push, Vector.getElem_append]
+        have h₅ : ↑i ≥ m := by omega
+        have h₆ : ↑i - m ≥ n := by omega
+        simp [h₄, h₆]
+    · have := Option.eq_none_iff_forall_ne_some.mpr h₂
+      have := exprOutputs'_finIdxOf?_none_to_exprOutputs this
+      simp [this, ← hvar_names]
+      split <;> rename_i h₃
+      · rfl
+      · simp [hlive_vars, SimR.varsToChans]
+        cases name with
+        | var var' pathConds' =>
+          simp
+          intros h
+          simp [h, compileExpr.varNames, compileExpr.varName] at h₃
+          simp [compileExpr.allVarsExcept, List.toVector] at h₁
+          split <;> rename_i h₄
+          · replace h₄ := (hdefined_vars var').mpr ⟨_, h₄⟩
+            have := h₁ (List.mem_to_mem_removeAll h₄ (by simp [h₃]))
+            simp [h] at this
+          · rfl
+        | merge_cond condName => rfl
+        | _ => simp [hexpr]
+
+end Wavelet.Simulation.Tail
